Coding.v
@@ -15,6 +15,8 @@ Definition binary alpha := bounded 2 alpha.
 
 Section Model.
 
+  Context {Δ0 : Delta0}.
+
   Variable D : Type.
   Variable I : interp D.
   Notation "⊨ phi" := (forall rho, rho ⊨ phi) (at level 21).
@@ -575,98 +577,5 @@ Section notStd.
 
 
 End notStd.
-
-
-Lemma LEM_binary phi : 
-  delta0 phi -> binary phi -> ⊨ ∀∀ phi ∨ ¬ phi.
-Proof.
-  intros delta0_phi binary_phi rho d e.
-  induction phi using form_ind_falsity_on.
-  - cbn. tauto.
-  - destruct P.
-  (* - apply inversion_bounded_bin in binary_phi.
-    apply inversion_delta0_bin in delta0_phi.
-    specialize (IHphi1 (fst delta0_phi) (proj1 binary_phi)).
-    specialize (IHphi2 (snd delta0_phi) (proj2 binary_phi) ).
-    destruct b.
-    all: fold sat in *; cbn in *; tauto.
-  - cbn. eapply Peano.eq_dec. apply axioms.
-  - inversion delta0_phi. *)
-Abort.
-
-
-Lemma LEM_bounded_exist_sat phi : 
-  delta0 phi -> binary phi -> ⊨ ∀∀ (∃ $0 ⧀ $2 ∧ phi) ∨ ¬ (∃ $0 ⧀ $2 ∧ phi).
-Proof.
-  (* intros delta0_phi binary_phi ρ N.
-  pose (Phi := ∀ (∃ $0 ⧀ $2 ∧ phi) ∨ ¬ (∃ $0 ⧀ $2 ∧ phi)).
-  assert (H : forall d rho, (d.:rho) ⊨ Phi).
-  apply induction. apply axioms.
-  repeat solve_bounds.
-  eapply bounded_up. apply binary_phi. lia.
-  eapply bounded_up. apply binary_phi. lia.
-  - intros rho y. cbn. right.
-    now intros (? & ?%nolessthen_zero & ?).
-  - intros n IHN rho y. cbn.
-    destruct (IHN rho y) as [IH|IH]; fold sat in *; cbn in IH.
-    + left. destruct IH as [d Hd]. exists d. split.
-      ++ destruct Hd as [[k ->] _]. exists (iσ k). 
-        now rewrite add_rec_r.
-      ++ eapply bound_ext. apply binary_phi.
-        2 : apply Hd.
-        intros [|[]]; solve_bounds.
-    + specialize (LEM_binary phi delta0_phi binary_phi) as lem_phi.
-      destruct (lem_phi (fun _ => i0) y n) as [HN|HN].
-      ++ left. exists n. split.
-        exists i0. now rewrite add_zero_r.
-        eapply bound_ext. apply binary_phi.
-        2 : apply HN.
-        intros [|[]]; solve_bounds.
-      ++ right. intros H. apply IH.
-        destruct H as (x & Hx1%lt_S & Hx2).
-        exists x. split.
-        destruct Hx1 as [| ->]. assumption.
-        exfalso. apply HN.
-        eapply bound_ext. apply binary_phi.
-        2 : apply Hx2.
-        intros [|[]]; solve_bounds.
-        eapply bound_ext. apply binary_phi.
-        2 : apply Hx2.
-        intros [|[]]; solve_bounds.
-        apply axioms.
-    - intros y. specialize (H N (fun _ => N) y).
-      fold sat in H; cbn in *. 
-      destruct H as [h|h].
-      left. destruct h as [d Hd]. 
-      exists d. split. apply Hd.
-      eapply bound_ext. apply binary_phi.
-      2 : apply Hd.
-      intros [|[]]; solve_bounds.
-      right. intros h1. apply h.
-      destruct h1 as [d Hd]. 
-      exists d. split. apply Hd.
-      eapply bound_ext. apply binary_phi.
-      2 : apply Hd.
-      intros [|[]]; solve_bounds. *)
-Abort.
-
-Corollary LEM_bounded_exist {phi} sigma : 
-  delta0 phi -> binary phi -> forall b x, (x .: b .: sigma) ⊨ (∃ $0 ⧀ $2 ∧ phi) \/ ~ (x .: b .: sigma) ⊨ (∃ $0 ⧀ $2 ∧ phi).
-Proof.
-  (* intros delta0_phi binary_phi b y.
-  specialize (LEM_bounded_exist_sat _ delta0_phi binary_phi) as Hb.
-  destruct (Hb (fun _ => b) b y) as [h|h]; fold sat in *; cbn in h.
-  left. destruct h as [d Hd].
-  exists d. split. apply Hd.
-  eapply bound_ext. apply binary_phi. 2 : apply Hd.
-  intros [|[]]; solve_bounds.
-  right. intros h1. apply h.
-  destruct h1 as [d Hd].
-  exists d. split. apply Hd.
-  eapply bound_ext. apply binary_phi. 2 : apply Hd.
-  intros [|[]]; solve_bounds. *)
-Abort.
-
-
 End Coding.
 End Model.
