Makholm.v
@@ -12,6 +12,8 @@ Notation "x ∣ y" := (exists k, x * k = y) (at level 50).
 
 Section Model.
 
+  Context {Δ0 : Delta0}.
+
   Variable D : Type.
   Variable I : interp D.
   Notation "⊨ phi" := (forall rho, rho ⊨ phi) (at level 21).
