WCT_Variants.v
@@ -7,6 +7,7 @@ Notation "⊨ phi" := (forall rho, rho ⊨ phi) (at level 21).
 Section Variants.
 
 Instance ff : falsity_flag := falsity_on.
+Context {Δ0 : Delta0}.
 
 Variable D : Type.
 Variable I : interp D.
@@ -107,7 +108,7 @@ Proof.
   assert (~ exists e, ~ std e) as He.
   apply (DN_remove (Irred_repr)).
   intros [ψ ].
-  { eapply Tennenbaum_diagonal' with (ψ:=ψ); eauto.
+  { eapply Tennenbaum_diagonal' with (ψ0:=ψ); eauto.
     now apply WCT_WRTs. }
   intros e. apply MP_Discrete_stable_std; auto.
   intros nH. apply He. now exists e.
